Changed bucketsort in boogie to really use buckets instead of comparison operation.

boogie/bucketsort.bpl
@@ -1,12 +1,13 @@
 // Define array type.
 type Array = [int] int;
+type ArrayArray = [int] Array;
 
 const N: int;
 axiom N > 0;
 
 function small_elements (a: Array, count: int) returns (bool)
 {
-  (forall i: int :: 0 <= i && i <= count ==> -3*N <= a [i] && a [i] <= 3*N)
+  (forall i: int :: 0 <= i && i < count ==> -3*N <= a [i] && a [i] < 3*N)
 }
 
 function is_permutation (perm: Array, count: int) returns (bool)
@@ -17,55 +18,131 @@ function is_permutation (perm: Array, count: int) returns (bool)
 
 function is_sorted (a: Array, count: int) returns (bool)
 {
-  (forall i,j: int :: 0 <= i && i < j && j <= count ==> a[i] <= a[j])
+  (forall i,j: int :: 0 <= i && i < j && j < count ==> a[i] <= a[j])
 }
 
 procedure BucketSort (input: Array, count: int) returns (result, permutation: Array)
   // Small elements.
-  requires small_elements (input, count); 
-  
+  requires small_elements (input, count);
+  requires count > 0;
+
   ensures small_elements (result, count);
   ensures is_sorted (result, count);
-  
+
   // Result is a permutation.
   ensures is_permutation (permutation, count);
   ensures (forall i:int :: 0 <= i && i < count ==> result [i] == input [permutation[i]]);
 {
-  var tmp, value: int;
+  var tmp, value, bucket_index: int;
   var left, middle, right: Array;
   var left_count, middle_count, right_count: int;
-  
+
+  var buckets: ArrayArray;
+  var counts: Array;
+
+
   tmp := 0;
   left_count := 0;
   middle_count := 0;
   right_count := 0;
-  
-  
-  while (tmp <= count)
+
+  counts [0] := 0;
+  counts [1] := 0;
+  counts [2] := 0;
+
+
+  while (tmp < count)
     invariant (forall i:int :: 0 <= i && i < tmp ==> permutation [i] == i && input [i] == result [i]);
+
     invariant (forall i: int :: 0 <= i && i < left_count ==> -3*N <= left [i] && left [i] < -N);
     invariant (forall i: int :: 0 <= i && i < middle_count ==> -N <= middle [i] && middle [i] <= N);
     invariant (forall i: int :: 0 <= i && i < right_count ==> N < right [i] && right [i] <= 3*N);
+    invariant left_count + middle_count + right_count  == tmp;
+
+    invariant (forall i: int :: 0 <= i && i < counts[0] ==> -3*N <= buckets[0] [i] && buckets[0] [i] < -N);
+    invariant (forall i: int :: 0 <= i && i < counts[1] ==> -N <= buckets[1] [i] && buckets[1] [i] < N);
+    invariant (forall i: int :: 0 <= i && i < counts[2] ==> N <= buckets[2] [i] && buckets[2] [i] < 3*N);
+    invariant counts [0] + counts [1] + counts [2]  == tmp;
+
+    invariant (forall i:int :: 0 <= i && i < 3 ==> 0 <= counts [i] && counts[i] <= count);
+
   {
     value := input [tmp];
+    bucket_index := (value + 3*N) div (2*N);
+
+    assert 0 <= bucket_index && bucket_index < 3;
+    assert bucket_index == 0 ==> -3*N <= value && value < -N;
+    assert bucket_index == 1 ==> -N <= value && value < N;
+    assert bucket_index == 2 ==> N <= value && value < 3*N;
+
+    buckets [bucket_index] [counts [bucket_index]] := value;
+    counts [bucket_index] := counts [bucket_index] + 1;
+
     if (value < -N) {
       left [left_count] := value;
       left_count := left_count + 1;
+    } else if (value <= N) {
+      middle [middle_count] := value;
+      middle_count := middle_count + 1;
     } else {
-      if (value <= N) {
-        middle [middle_count] := value;
-        middle_count := middle_count + 1;
-      } else {
-        right [right_count] := value;
-        right_count := right_count + 1;
-      }
+      right [right_count] := value;
+      right_count := right_count + 1;
     }
-    
+
     permutation [tmp] := tmp;
     result [tmp] := input [tmp];
     tmp := tmp + 1;
   }
-  
-  
-  
+
+  // Individual sort algorithms.
+  //call left := MagicSort (left, left_count, -3*N, -N-1);
+  //call middle := MagicSort (middle, middle_count, -N, N);
+  //call right := MagicSort (right, right_count, N+1, 3*N);
+
+  left_count := counts [0];
+  middle_count := counts [1];
+  right_count := counts [2];
+
+  call left := MagicSort (buckets [0], counts [0], -3*N, -N-1);
+  call middle := MagicSort (buckets [1], counts [1], -N, N-1);
+  call right := MagicSort (buckets [2], counts [2], N, 3*N-1);
+
+  // Concatenate arrays.
+  tmp := 0;
+  while (tmp < left_count)
+    invariant small_elements (result, tmp);
+    invariant is_sorted (result, tmp);
+    invariant (forall i:int :: 0 <= i && i < tmp ==> result [i] == left [i]);
+    invariant tmp <= left_count;
+  {
+    result [tmp] := left [tmp];
+    tmp := tmp + 1;
+  }
+
+  while (tmp < left_count + middle_count)
+    invariant small_elements (result, tmp);
+    invariant is_sorted (result, tmp);
+    invariant (forall i:int :: 0 <= i && i < left_count ==> result [i] == left [i]);
+    invariant (forall i:int :: left_count <= i && i < tmp ==> result [i] == middle [i-left_count]);
+    invariant tmp <= left_count+middle_count;
+  {
+    result [tmp] := middle [tmp-left_count];
+  }
+
+  while (tmp < left_count + middle_count + right_count)
+    invariant small_elements (result, tmp);
+    invariant is_sorted (result, tmp);
+    invariant (forall i:int :: 0 <= i && i < left_count ==> result [i] == left [i]);
+    invariant (forall i:int :: left_count <= i && i < left_count + middle_count ==> result [i] == middle [i-left_count]);
+    invariant (forall i:int :: left_count + middle_count <= i && i < tmp ==> result [i] == middle [i-left_count-middle_count]);
+    invariant tmp <= left_count+middle_count;
+  {
+    result [tmp] := middle [tmp-left_count];
+  }
 }
+
+procedure MagicSort (input: Array, count: int, lower_bound, upper_bound: int) returns (output: Array);
+  requires (forall i:int :: 0 <= i && i < count ==> lower_bound <= input [i] && input [i] <= upper_bound);
+  ensures is_sorted (output, count);
+  ensures (forall i:int :: 0 <= i && i < count ==> lower_bound <= output [i] && output [i] <= upper_bound);
+
